## 3 terms, first coefficient $= 1$

$$\Large x^2+7x+12$$

Find two numbers that **multiply to the third** coefficient and **sum to the second**.

In this case they should multiply to 12 and sum to 7.

Once you find them, write the equation in this way:

$$\Large (x+3)(x+4)$$

## 3 terms, first coefficient $\neq 1$

$$\Large 2x^2-6x -56$$

Try to **make the first coefficient 1**, then solve as above.

$$\Large 2(x^2-3x-28)$$
$$\Large 2(x+4)(x-7)$$

## Squared binomials

### Difference of perfect squares

$$\Large x^2-16$$
Take the **square root of both numbers** and write the equation like this:

$$\Large(x+6)(x-6)$$
**One will be positive** and **one will be negative**.


## Quadratic formula

If you are too retarded to solve one of these, use the quadratic formula:

$$\Large x=\frac{−b±\sqrt{b^2−4ac}}{2a}$$

> [!example]
> $$\Large 2x^2-6x -56$$
> $$\Large x=\frac{+6±\sqrt{36+448}}{4}$$
> $$\Large x= \frac{+6±22}{4}$$
> $$\Large x=\frac{6 + 22}{4};\quad x=\frac{6-22}{4}$$
> $$\Large x=\frac{28}{4};\quad x=\frac{-16}{4}$$
> $$\Large x=7;\quad x= -4$$
