> [!example]
> $$\large \frac{(x-1)(x^2-4x+4)}{x-3}>=0$$
> 
> $x-1 >= 0 \quad <=> \quad x>=1 \quad <=> \quad x\in [1,+\inf)$
> $x^2-4x+4>=0 \quad <=> \quad x \in \mathbb{R}=(-\inf, +\inf)$ (equal to $(a+b)^2$? which is always positive.
> $x-3>0 \quad <=> \quad x > 3 \quad <=> \quad x \in (3, +\inf)$
> 
> ![](../z_images/20241008_084917%201.jpg)

> [!example]
> $$\large x+2>=^3\sqrt{x+2}$$
> 
> $A>= \sqrt{B}^3 \quad <=> \quad A^3 >= (^3\sqrt{B})^3$
> $(x+2)^3 >= (x+2)$ (the original inequality is equal to this one)
> $(x+2)((x+2)^2-1)>=0$
> $(x+2)(x+3)(x+1)$
> ![](../z_images/Pasted%20image%2020241008090316.png)
> 
> $$\large x \in [-3, -2]\cup [-1, +\inf)$$
> 
> $a^3-b^3=(a-b)(a^2+ab+b^2) \qquad \forall a,b \in \mathbb{R}$
> ???

> [!example]
> $$\large \frac{x-\sqrt{x+2}}{x^2-3x+2}>0$$
> $A=x-\sqrt{x+2}>=0$
> $B=x^2-3x+2>0 \quad \Rightarrow \quad (x-1)(x-2)$
> 
> $\large B>0$
> ![](../z_images/Pasted%20image%2020241008091605.png)
> $B>0 \quad <=> \quad x \in (-\inf, 1)\cup(2,+\inf)$
> 
> $\large A>=0$
> 
> $x>=\sqrt{x+2}$ (right side is positive for sure, but left side we are not sure)
> 
> $\begin{cases} x+2>= 0 \\ x>= 0 \\ x^2>=(^2\sqrt{x+2})^2\end{cases} \quad \Rightarrow \quad \begin{cases} x\in [-2,+\infty) \\ x \in [0, +\infty) \\ x^2-x-2>=0\end{cases}$
> 
> $x=\frac{1+-\sqrt{1+8}}{2}=\frac{1+-3}{2} = -2 \quad \& \quad 1$
> $x^2-x-2=(x+1)(x-2)>=0 \quad <=> \quad x\in \underbracket{(-\infty, 1)}_{\text{not needed}}\cup[2, +\infty)$
> 
> $A>=0 \quad <=> \quad x\in[2, +\infty)$
> 
> $\large \frac{A}{B}>=0$
> ![](../z_images/Pasted%20image%2020241008092926.png)
> 
> $\frac{A}{B}>=0 \quad <=> \quad x \in (1, 2) \cup (2, +\infty)$
> 
> > [!hint]
> In 
> $$\large a^2-b^2=\underbracket{(a+b)}_{>=0}(a-b)$$
> $(a+b)$ is always positive, so we don't take it into account while computing the sign.

